src/Compile/Simulation/Simulation_Preservation.thy
@@ -86,13 +86,13 @@ text \<open>A single \<^const>\<open>pstep\<close> touches only the head region 
   bridges the \<open>Nested\<close> snoc (the inner step threads all frames) to the induction hypothesis
   (stated on the inner frames alone).\<close>
 lemma pstep_frame_restrict:
-  "pstep source_global \<Pi> (c, s, fr) (c', s', frs') \<Longrightarrow> fr = frs @ extra \<Longrightarrow> frs \<noteq> [] \<Longrightarrow>
-   \<exists>frs''. frs' = frs'' @ extra \<and> pstep source_global \<Pi> (c, s, frs) (c', s', frs'')"
+  "pstep gs \<Pi> (c, s, fr) (c', s', frs') \<Longrightarrow> fr = frs @ extra \<Longrightarrow> frs \<noteq> [] \<Longrightarrow>
+   \<exists>frs''. frs' = frs'' @ extra \<and> pstep gs \<Pi> (c, s, frs) (c', s', frs'')"
 proof (induction "(c, s, fr)" "(c', s', frs')"
        arbitrary: c s fr frs c' s' frs' rule: pstep.induct)
   case (Seq2 c1 s1 f1 c1' s1' f1' c2 frs)
   from Seq2.hyps(2)[OF Seq2.prems] obtain frs'' where
-    ih: "f1' = frs'' @ extra" "pstep source_global \<Pi> (c1, s1, frs) (c1', s1', frs'')" by blast
+    ih: "f1' = frs'' @ extra" "pstep gs \<Pi> (c1, s1, frs) (c1', s1', frs'')" by blast
   show ?case
     by (rule exI[of _ frs'']) (use ih in auto)
 next
@@ -114,14 +114,14 @@ text \<open>Unlike \<open>pstep_frame_restrict\<close> this needs no non-empty a
   command never heads with \<^const>\<open>SKIP\<close> / \<^const>\<open>Restore\<close> / \<^const>\<open>Unwind\<close>, so no pop can
   fire.\<close>
 lemma pstep_call_frame_restrict:
-  "pstep source_global \<Pi> (c, s, fr) (c', s', frs') \<Longrightarrow> head_call c \<Longrightarrow> fr = frs @ extra \<Longrightarrow>
-   \<exists>frs''. frs' = frs'' @ extra \<and> pstep source_global \<Pi> (c, s, frs) (c', s', frs'')"
+  "pstep gs \<Pi> (c, s, fr) (c', s', frs') \<Longrightarrow> head_call c \<Longrightarrow> fr = frs @ extra \<Longrightarrow>
+   \<exists>frs''. frs' = frs'' @ extra \<and> pstep gs \<Pi> (c, s, frs) (c', s', frs'')"
 proof (induction "(c, s, fr)" "(c', s', frs')"
        arbitrary: c s fr frs c' s' frs' rule: pstep.induct)
   case (Seq2 c1 s1 f1 c1' s1' f1' c2 frs)
   from Seq2.prems(1) have "head_call c1" by simp
   from Seq2.hyps(2)[OF this Seq2.prems(2)] obtain frs'' where
-    ih: "f1' = frs'' @ extra" "pstep source_global \<Pi> (c1, s1, frs) (c1', s1', frs'')" by blast
+    ih: "f1' = frs'' @ extra" "pstep gs \<Pi> (c1, s1, frs) (c1', s1', frs'')" by blast
   show ?case by (rule exI[of _ frs'']) (use ih in auto)
 next
   case (Call p decl actuals dst vals callee s1 frs0 frs)
@@ -132,13 +132,13 @@ text \<open>The CFG dual: a \<^const>\<open>cstep\<close> also touches only the 
   bottom segment rides along --- with no non-emptiness needed, since the return step already
   requires a non-empty stack.\<close>
 lemma cstep_frame_extend:
-  "cstep source_global g (u, s, stk) (u', s', stk') \<Longrightarrow>
-   cstep source_global g (u, s, stk @ E) (u', s', stk' @ E)"
+  "cstep gs g (u, s, stk) (u', s', stk') \<Longrightarrow>
+   cstep gs g (u, s, stk @ E) (u', s', stk' @ E)"
   by (erule cstep.cases) auto
 
 lemma cstep_star_frame_extend:
-  assumes "star (cstep source_global g) c c'"
-  shows "star (cstep source_global g) (fst c, fst (snd c), snd (snd c) @ E)
+  assumes "star (cstep gs g) c c'"
+  shows "star (cstep gs g) (fst c, fst (snd c), snd (snd c) @ E)
                         (fst c', fst (snd c'), snd (snd c') @ E)"
   using assms
 proof (induction rule: star.induct)
@@ -147,8 +147,8 @@ next
   case (step a b c)
   obtain ua sa stka where a: "a = (ua, sa, stka)" by (cases a)
   obtain ub sb stkb where b: "b = (ub, sb, stkb)" by (cases b)
-  from step.hyps(1) a b have "cstep source_global g (ua, sa, stka) (ub, sb, stkb)" by simp
-  hence "cstep source_global g (ua, sa, stka @ E) (ub, sb, stkb @ E)" by (rule cstep_frame_extend)
+  from step.hyps(1) a b have "cstep gs g (ua, sa, stka) (ub, sb, stkb)" by simp
+  hence "cstep gs g (ua, sa, stka @ E) (ub, sb, stkb @ E)" by (rule cstep_frame_extend)
   with step.IH a b show ?case by (auto intro: star.step)
 qed
 
@@ -156,18 +156,18 @@ text \<open>The \<open>Nested\<close> step-inversion rule: stepping a wrapped ac
   \<^term>\<open>Seq inner Restore\<close> is stepping \<open>inner\<close>, provided \<open>inner\<close> has neither completed nor
   begun to unwind (either of which would relocate rather than step).\<close>
 lemma pstep_seq_after_seq_restore:
-  assumes step: "pstep source_global \<Pi> (seq_after (Seq inner Restore) afters, s, frs) src'"
+  assumes step: "pstep gs \<Pi> (seq_after (Seq inner Restore) afters, s, frs) src'"
       and nsk: "inner \<noteq> SKIP" and nunw: "inner \<noteq> Unwind"
   obtains inner' s' fz where
     "src' = (seq_after (Seq inner' Restore) afters, s', fz)"
-    "pstep source_global \<Pi> (inner, s, frs) (inner', s', fz)"
+    "pstep gs \<Pi> (inner, s, frs) (inner', s', fz)"
 proof -
   obtain h' s' fz where
     src': "src' = (seq_after h' afters, s', fz)"
-      and hstep: "pstep source_global \<Pi> (Seq inner Restore, s, frs) (h', s', fz)"
+      and hstep: "pstep gs \<Pi> (Seq inner Restore, s, frs) (h', s', fz)"
     by (rule pstep_seq_after_headE[OF step]) auto
   from hstep nsk nunw obtain inner' where
-    "h' = Seq inner' Restore" "pstep source_global \<Pi> (inner, s, frs) (inner', s', fz)"
+    "h' = Seq inner' Restore" "pstep gs \<Pi> (inner, s, frs) (inner', s', fz)"
     by auto
   with src' show ?thesis using that by blast
 qed
@@ -186,14 +186,14 @@ lemma csim_call_base:
       and loc: "control_at \<Pi> p c0 kk n (seq_after (Call dst q actuals) afters) v"
       and cacc: "compiled_at \<Pi> g p c0 kk n"
       and decl: "\<Pi> q = Some decl"
-  shows "\<exists>cfg'. star (cstep source_global g) (v, s, [])  cfg'
+  shows "\<exists>cfg'. star (cstep gs g) (v, s, [])  cfg'
               \<and> csim \<Pi> g (seq_after (Seq (body decl) Restore) afters,
                           bind_formals (formals decl) (map (\<lambda>e. aval e s) actuals)
-                            (enter_state source_global s),
+                            (enter_state gs s),
                           [Frame s dst]) cfg'"
 proof -
   let ?callee =
-    "bind_formals (formals decl) (map (\<lambda>e. aval e s) actuals) (enter_state source_global s)"
+    "bind_formals (formals decl) (map (\<lambda>e. aval e s) actuals) (enter_state gs s)"
   have spNone: "special_table q = None" by (rule procs_embedded_special_table_none[OF pc decl])
   from cacc obtain n' en E K where comp: "compile \<Pi> p c0 kk n = (n', en, E, K)"
       and Ksub: "K \<subseteq> calls g" by blast
@@ -204,20 +204,20 @@ proof -
     and callerSKIP: "control_at \<Pi> p c0 kk n (seq_after SKIP afters) w" by blast
   have edge: "(Statement j, CallEdge dst (formals decl) actuals, FunctionEntry q, w)
                 \<in> calls g" using edgeK Ksub by (auto simp: decl)
-  have cstep1: "cstep source_global g (Statement j, s, [])
-           (FunctionEntry q, call_enter source_global (CallEdge dst (formals decl) actuals) s,
+  have cstep1: "cstep gs g (Statement j, s, [])
+           (FunctionEntry q, call_enter gs (CallEdge dst (formals decl) actuals) s,
             [(w, dst, s)])" by (rule cstep.Call[OF edge])
-  have ce: "call_enter source_global (CallEdge dst (formals decl) actuals) s = ?callee"
+  have ce: "call_enter gs (CallEdge dst (formals decl) actuals) s = ?callee"
     by (rule call_enter_CallEdge)
   obtain kq m en_q where
     caccq: "compiled_at \<Pi> g q (body decl) kq m"
       and ctrlq: "control_at \<Pi> q (body decl) kq m (body decl) en_q"
       and entry: "(FunctionEntry q, EA_Nop, en_q) \<in> intra g"
     by (rule procs_embedded_activation[OF pc decl])
-  have cstep2: "cstep source_global g (FunctionEntry q, ?callee, [(w, dst, s)])
+  have cstep2: "cstep gs g (FunctionEntry q, ?callee, [(w, dst, s)])
                         (en_q, ?callee, [(w, dst, s)])"
     using cstep_nop[OF entry] .
-  have star: "star (cstep source_global g) (v, s, []) (en_q, ?callee, [(w, dst, s)])"
+  have star: "star (cstep gs g) (v, s, []) (en_q, ?callee, [(w, dst, s)])"
     using cstep1[unfolded ce] cstep2 vk by (simp add: star.step)
   have baseCallee: "csim \<Pi> g (body decl, ?callee, []) (en_q, ?callee, [])"
     by (rule csim.Base[OF ctrlq caccq])
@@ -231,36 +231,36 @@ qed
 
 theorem csim_call_completion:
   "csim \<Pi> g (c, s, frs) (v, t, stk) \<Longrightarrow> procs_embedded \<Pi> g \<Longrightarrow> head_call c \<Longrightarrow>
-   pstep source_global \<Pi> (c, s, frs) src' \<Longrightarrow>
-   \<exists>cfg'. star (cstep source_global g) (v, t, stk) cfg' \<and> csim \<Pi> g src' cfg'"
+   pstep gs \<Pi> (c, s, frs) src' \<Longrightarrow>
+   \<exists>cfg'. star (cstep gs g) (v, t, stk) cfg' \<and> csim \<Pi> g src' cfg'"
 proof (induction "(c, s, frs)" "(v, t, stk)" arbitrary: c s frs v t stk src' rule: csim.induct)
   case (Base p c0 kk n cc vv ss)
   from head_call_seq_after_form[OF Base.prems(2)] obtain dst q actuals afters where
     ceq: "cc = seq_after (Call dst q actuals) afters" and spNone: "special_table q = None"
     by blast
-  have step: "pstep source_global \<Pi> (seq_after (Call dst q actuals) afters, ss, []) src'"
+  have step: "pstep gs \<Pi> (seq_after (Call dst q actuals) afters, ss, []) src'"
     using Base.prems(3) ceq by simp
   have w1: "Call dst q actuals \<noteq> SKIP" by simp
   have w2: "Call dst q actuals \<noteq> Unwind" by simp
   obtain h' s' fz where
     src': "src' = (seq_after h' afters, s', fz)"
-      and pcall: "pstep source_global \<Pi> (Call dst q actuals, ss, []) (h', s', fz)"
+      and pcall: "pstep gs \<Pi> (Call dst q actuals, ss, []) (h', s', fz)"
     by (rule pstep_seq_after_headE[OF step w1 w2])
   from pcall spNone obtain decl where
     qdecl: "\<Pi> q = Some decl"
       and heq: "h' = Seq (body decl) Restore"
       and seq: "s' = bind_formals (formals decl) (map (\<lambda>e. aval e ss) actuals)
-                        (enter_state source_global ss)"
+                        (enter_state gs ss)"
       and fzeq: "fz = [Frame ss dst]"
     by auto
   have loc': "control_at \<Pi> p c0 kk n (seq_after (Call dst q actuals) afters) vv"
     using Base.hyps(1) ceq by simp
   from csim_call_base[OF Base.prems(1) loc' Base.hyps(2) qdecl, where s = ss]
   obtain cfg' where
-    cstar: "star (cstep source_global g) (vv, ss, []) cfg'"
+    cstar: "star (cstep gs g) (vv, ss, []) cfg'"
       and csimr: "csim \<Pi> g (seq_after (Seq (body decl) Restore) afters,
                bind_formals (formals decl) (map (\<lambda>e. aval e ss) actuals)
-                 (enter_state source_global ss),
+                 (enter_state gs ss),
                [Frame ss dst]) cfg'" by blast
   from csimr have "csim \<Pi> g src' cfg'" by (simp add: src' heq seq fzeq)
   with cstar show ?case by blast
@@ -275,16 +275,16 @@ next
   have nunw: "inner \<noteq> Unwind" using headinner by (rule head_call_not_Unwind)
   obtain inner' s' fz where
     src': "src' = (seq_after (Seq inner' Restore) afters, s', fz)"
-      and stepin: "pstep source_global \<Pi> (inner, s0, frs0 @ [Frame caller dst]) (inner', s', fz)"
+      and stepin: "pstep gs \<Pi> (inner, s0, frs0 @ [Frame caller dst]) (inner', s', fz)"
     by (rule pstep_seq_after_seq_restore[OF Nested.prems(3) nsk nunw])
   from pstep_call_frame_restrict[OF stepin headinner refl] obtain fz' where
     fz: "fz = fz' @ [Frame caller dst]"
-      and stepin': "pstep source_global \<Pi> (inner, s0, frs0) (inner', s', fz')" by blast
+      and stepin': "pstep gs \<Pi> (inner, s0, frs0) (inner', s', fz')" by blast
   from Nested.hyps(2)[OF Nested.prems(1) headinner stepin'] obtain v' t' stk' where
-    cstepin: "star (cstep source_global g) (v0, s0, stk0) (v', t', stk')"
+    cstepin: "star (cstep gs g) (v0, s0, stk0) (v', t', stk')"
       and csimin: "csim \<Pi> g (inner', s', fz') (v', t', stk')" by auto
   have teq: "t' = s'" using csim_store_eq[OF csimin] by simp
-  have cstepN: "star (cstep source_global g) (v0, s0, stk0 @ [(cont, dst, caller)])
+  have cstepN: "star (cstep gs g) (v0, s0, stk0 @ [(cont, dst, caller)])
                                (v', s', stk' @ [(cont, dst, caller)])"
     using cstep_star_frame_extend[OF cstepin, of "[(cont, dst, caller)]"] teq by simp
   have "csim \<Pi> g (seq_after (Seq inner' Restore) afters, s', fz' @ [Frame caller dst])
@@ -337,7 +337,7 @@ text \<open>
 theorem csim_intra_completion:
   "csim \<Pi> g (c, s, frs) (v, t, stk) \<Longrightarrow> procs_embedded \<Pi> g \<Longrightarrow>
    intra_step \<Pi> (c, s, frs) src' \<Longrightarrow>
-   \<exists>cfg'. star (cstep source_global g) (v, t, stk) cfg' \<and> csim \<Pi> g src' cfg'"
+   \<exists>cfg'. star (cstep gs g) (v, t, stk) cfg' \<and> csim \<Pi> g src' cfg'"
 proof (induction "(c, s, frs)" "(v, t, stk)" arbitrary: c s frs v t stk src' rule: csim.induct)
   case (Base p c0 kk n cc vv ss)
   obtain c' s' frs' where sc: "src' = (c', s', frs')" by (cases src')
@@ -351,7 +351,7 @@ proof (induction "(c, s, frs)" "(v, t, stk)" arbitrary: c s frs v t stk src' rul
       and Esub: "E \<subseteq> intra g" by blast
   from intra_step_simulation[OF Base.hyps(1) istep comp Esub srcbody, where stk = "[]"]
   obtain v' where feq: "frs' = []" and loc': "control_at \<Pi> p c0 kk n c' v'"
-      and cstar: "star (cstep source_global g) (vv, ss, []) (v', s', [])" by blast
+      and cstar: "star (cstep gs g) (vv, ss, []) (v', s', [])" by blast
   have "csim \<Pi> g (c', s', []) (v', s', [])" by (rule csim.Base[OF loc' Base.hyps(2)])
   with cstar show ?case using sc feq by auto
 next
@@ -381,13 +381,13 @@ next
       and Esub: "E \<subseteq> intra g"
       and exitedge: "(kin, EA_Ret None pin, FunctionResult pin) \<in> intra g"
       using ftin by blast
-    have star1: "star (cstep source_global g) (v0, s0, [(cont, dst, caller)])
+    have star1: "star (cstep gs g) (v0, s0, [(cont, dst, caller)])
                    (kin, s0, [(cont, dst, caller)])"
       by (rule control_at_skip_to_exit[OF ctrl refl comp Esub])
-    have "cstep source_global g (kin, s0, [(cont, dst, caller)])
+    have "cstep gs g (kin, s0, [(cont, dst, caller)])
             (FunctionResult pin, s0, [(cont, dst, caller)])"
       using cstep.Intra[OF exitedge edge_step_EA_Ret_ret_store_mem] by simp
-    with star1 have star: "star (cstep source_global g) (v0, s0, [(cont, dst, caller)])
+    with star1 have star: "star (cstep gs g) (v0, s0, [(cont, dst, caller)])
                              (FunctionResult pin, s0, [(cont, dst, caller)])"
       by (rule star_trans[OF _ star_step1])
     have "csim \<Pi> g (seq_after Restore afters, s0, [Frame caller dst])
@@ -409,10 +409,10 @@ next
     from intra_step_any_frame[OF stepin]
     have stepin': "intra_step \<Pi> (inner, s0, frs0) (inner', s', frs0)" .
     from Nested.hyps(2)[OF Nested.prems(1) stepin'] obtain v' t' stk' where
-      cstepin: "star (cstep source_global g) (v0, s0, stk0) (v', t', stk')"
+      cstepin: "star (cstep gs g) (v0, s0, stk0) (v', t', stk')"
         and csimin: "csim \<Pi> g (inner', s', frs0) (v', t', stk')" by auto
     have teq: "t' = s'" using csim_store_eq[OF csimin] by simp
-    have cstepN: "star (cstep source_global g) (v0, s0, stk0 @ [(cont, dst, caller)])
+    have cstepN: "star (cstep gs g) (v0, s0, stk0 @ [(cont, dst, caller)])
                                  (v', s', stk' @ [(cont, dst, caller)])"
       using cstep_star_frame_extend[OF cstepin, of "[(cont, dst, caller)]"] teq by simp
     have "csim \<Pi> g (seq_after (Seq inner' Restore) afters, s', frs0 @ [Frame caller dst])
@@ -436,8 +436,8 @@ text \<open>
 \<close>
 theorem csim_return_init_completion:
   "csim \<Pi> g (c, s, frs) (v, t, stk) \<Longrightarrow> procs_embedded \<Pi> g \<Longrightarrow> frs \<noteq> [] \<Longrightarrow>
-   head_return c \<Longrightarrow> pstep source_global \<Pi> (c, s, frs) src' \<Longrightarrow>
-   \<exists>cfg'. star (cstep source_global g) (v, t, stk) cfg' \<and> csim \<Pi> g src' cfg'"
+   head_return c \<Longrightarrow> pstep gs \<Pi> (c, s, frs) src' \<Longrightarrow>
+   \<exists>cfg'. star (cstep gs g) (v, t, stk) cfg' \<and> csim \<Pi> g src' cfg'"
 proof (induction "(c, s, frs)" "(v, t, stk)" arbitrary: c s frs v t stk src' rule: csim.induct)
   case (Base p c0 kk n cc vv ss)
   from Base.prems(2) show ?case by simp
@@ -452,7 +452,7 @@ next
   have nunw: "inner \<noteq> Unwind" using hr_inner by auto
   obtain inner' s' fz where
     src': "src' = (seq_after (Seq inner' Restore) afters, s', fz)"
-      and stepin: "pstep source_global \<Pi> (inner, s0, frs0 @ [Frame caller dst]) (inner', s', fz)"
+      and stepin: "pstep gs \<Pi> (inner, s0, frs0 @ [Frame caller dst]) (inner', s', fz)"
     by (rule pstep_seq_after_seq_restore[OF Nested.prems(4) nsk nunw])
   show ?case
   proof (cases "frs0 = []")
@@ -472,11 +472,11 @@ next
     obtain e cafters where innerform: "inner = seq_after (Return e) cafters"
       using head_return_seq_after_form[OF hr_inner] by blast
     \<comment> \<open>the head step is @{text \<open>Return e --> Unwind\<close>}, leaving the continuations \<open>cafters\<close>\<close>
-    have stepin1: "pstep source_global \<Pi> (seq_after (Return e) cafters, s0, [Frame caller dst])
+    have stepin1: "pstep gs \<Pi> (seq_after (Return e) cafters, s0, [Frame caller dst])
                      (inner', s', fz)"
       using stepin True innerform by simp
     obtain h' where inner'form: "inner' = seq_after h' cafters"
-        and hstep: "pstep source_global \<Pi> (Return e, s0, [Frame caller dst]) (h', s', fz)"
+        and hstep: "pstep gs \<Pi> (Return e, s0, [Frame caller dst]) (h', s', fz)"
       by (rule pstep_seq_after_headE[OF stepin1]) auto
     have hUnw: "h' = Unwind" and s'eq: "s' = ret_store e s0" and fzeq: "fz = [Frame caller dst]"
       using hstep by (cases e; auto simp: ret_store_def)+
@@ -493,7 +493,7 @@ next
       using control_at_seq_after_return_edge[OF ctrl[unfolded innerform] refl comp] by blast
     have edgeg: "(Statement j, EA_Ret e pin, FunctionResult pin) \<in> intra g"
       using edge Esub by blast
-    have cstep1: "cstep source_global g (Statement j, s0, [(cont, dst, caller)])
+    have cstep1: "cstep gs g (Statement j, s0, [(cont, dst, caller)])
                           (FunctionResult pin, ret_store e s0, [(cont, dst, caller)])"
       using cstep.Intra[OF edgeg edge_step_EA_Ret_ret_store_mem] .
     \<comment> \<open>the enclosing wrapper becomes @{text Returning}\<close>
@@ -505,7 +505,7 @@ next
     have srcshape: "src' = (seq_after (Seq (seq_after Unwind cafters) Restore) afters,
                             ret_store e s0, [Frame caller dst])"
       using src' inner'form hUnw s'eq fzeq by simp
-    have "star (cstep source_global g) (v0, s0, stk0 @ [(cont, dst, caller)])
+    have "star (cstep gs g) (v0, s0, stk0 @ [(cont, dst, caller)])
                          (FunctionResult pin, ret_store e s0, [(cont, dst, caller)])"
       using cstep1 vk stk0nil by auto
     with rel srcshape show ?thesis by auto
@@ -513,12 +513,12 @@ next
     case False
     from pstep_frame_restrict[OF stepin refl False] obtain fz' where
       fz: "fz = fz' @ [Frame caller dst]"
-        and stepin': "pstep source_global \<Pi> (inner, s0, frs0) (inner', s', fz')" by blast
+        and stepin': "pstep gs \<Pi> (inner, s0, frs0) (inner', s', fz')" by blast
     from Nested.hyps(2)[OF Nested.prems(1) False hr_inner stepin'] obtain v' t' stk' where
-      cstepin: "star (cstep source_global g) (v0, s0, stk0) (v', t', stk')"
+      cstepin: "star (cstep gs g) (v0, s0, stk0) (v', t', stk')"
         and csimin: "csim \<Pi> g (inner', s', fz') (v', t', stk')" by auto
     have teq: "t' = s'" using csim_store_eq[OF csimin] by simp
-    have cstepN: "star (cstep source_global g) (v0, s0, stk0 @ [(cont, dst, caller)])
+    have cstepN: "star (cstep gs g) (v0, s0, stk0 @ [(cont, dst, caller)])
                                  (v', s', stk' @ [(cont, dst, caller)])"
       using cstep_star_frame_extend[OF cstepin, of "[(cont, dst, caller)]"] teq by simp
     have "csim \<Pi> g (seq_after (Seq inner' Restore) afters, s', fz' @ [Frame caller dst])
@@ -552,24 +552,24 @@ lemma csim_returning_base_completion:
   assumes pr: "pop_ready w"
       and loc: "control_at \<Pi> pc c0c kc nc (seq_after SKIP afters) cont"
       and cacc: "compiled_at \<Pi> g pc c0c kc nc"
-      and step: "pstep source_global \<Pi> (seq_after w afters, callee, [Frame caller dst]) src'"
-  shows "\<exists>cfg'. star (cstep source_global g) (FunctionResult p, callee, [(cont, dst, caller)]) cfg'
+      and step: "pstep gs \<Pi> (seq_after w afters, callee, [Frame caller dst]) src'"
+  shows "\<exists>cfg'. star (cstep gs g) (FunctionResult p, callee, [(cont, dst, caller)]) cfg'
               \<and> csim \<Pi> g src' cfg'"
 proof -
   have wsk: "w \<noteq> SKIP" using pr by (rule pop_ready_not_SKIP)
   have wunw: "w \<noteq> Unwind" using pr by (rule pop_ready_not_Unwind)
   obtain h' s' frs' where
     src': "src' = (seq_after h' afters, s', frs')"
-      and hstep: "pstep source_global \<Pi> (w, callee, [Frame caller dst]) (h', s', frs')"
+      and hstep: "pstep gs \<Pi> (w, callee, [Frame caller dst]) (h', s', frs')"
     by (rule pstep_seq_after_headE[OF step wsk wunw])
-  let ?rs = "combine_collect source_global dst caller callee"
+  let ?rs = "combine_collect gs dst caller callee"
   from pstep_pop_ready_head[OF pr hstep] show ?thesis
   proof (rule disjE)
     assume "(h', s', frs') =
-              (SKIP, combine_assign dst (callee ret_var) (combine_env source_global caller callee),
+              (SKIP, combine_assign dst (callee ret_var) (combine_env gs caller callee),
                [])"
     hence h': "h' = SKIP" "s' = ?rs" "frs' = []" by (auto simp: combine_collect_def)
-    have "cstep source_global g (FunctionResult p, callee, [(cont, dst, caller)]) (cont, ?rs, [])"
+    have "cstep gs g (FunctionResult p, callee, [(cont, dst, caller)]) (cont, ?rs, [])"
       by (rule cstep.Return)
     moreover have "csim \<Pi> g (seq_after SKIP afters, ?rs, []) (cont, ?rs, [])"
       by (rule csim.Base[OF loc cacc])
@@ -590,8 +590,8 @@ text \<open>Deep return completion: the base case above, threaded out through an
   certificates \<open>csim\<close> already carries.\<close>
 theorem csim_returning_completion:
   "csim \<Pi> g (c, s, frs) (v, t, stk) \<Longrightarrow> is_returning c \<Longrightarrow>
-   pstep source_global \<Pi> (c, s, frs) src' \<Longrightarrow>
-   \<exists>cfg'. star (cstep source_global g) (v, t, stk) cfg' \<and> csim \<Pi> g src' cfg'"
+   pstep gs \<Pi> (c, s, frs) src' \<Longrightarrow>
+   \<exists>cfg'. star (cstep gs g) (v, t, stk) cfg' \<and> csim \<Pi> g src' cfg'"
 proof (induction "(c, s, frs)" "(v, t, stk)" arbitrary: c s frs v t stk src' rule: csim.induct)
   case (Base p c0 kk n cc vv ss)
   from control_at_not_returning[OF Base.hyps(1)] Base.prems(1) show ?case by simp
@@ -613,16 +613,16 @@ next
     using csim_returning_frames_nonempty[OF Nested.hyps(1) retinner] by simp
   obtain inner' s' fz where
     src': "src' = (seq_after (Seq inner' Restore) afters, s', fz)"
-      and stepin: "pstep source_global \<Pi> (inner, s0, frs0 @ [Frame caller dst]) (inner', s', fz)"
+      and stepin: "pstep gs \<Pi> (inner, s0, frs0 @ [Frame caller dst]) (inner', s', fz)"
     by (rule pstep_seq_after_seq_restore[OF Nested.prems(2) nsk nunw])
   from pstep_frame_restrict[OF stepin refl frsne] obtain fz' where
     fz: "fz = fz' @ [Frame caller dst]"
-      and stepin': "pstep source_global \<Pi> (inner, s0, frs0) (inner', s', fz')" by blast
+      and stepin': "pstep gs \<Pi> (inner, s0, frs0) (inner', s', fz')" by blast
   from Nested.hyps(2)[OF retinner stepin'] obtain v' t' stk' where
-    cstepin: "star (cstep source_global g) (v0, s0, stk0) (v', t', stk')"
+    cstepin: "star (cstep gs g) (v0, s0, stk0) (v', t', stk')"
       and csimin: "csim \<Pi> g (inner', s', fz') (v', t', stk')" by auto
   have teq: "t' = s'" using csim_store_eq[OF csimin] by simp
-  have cstepN: "star (cstep source_global g) (v0, s0, stk0 @ [(cont, dst, caller)])
+  have cstepN: "star (cstep gs g) (v0, s0, stk0 @ [(cont, dst, caller)])
                                (v', s', stk' @ [(cont, dst, caller)])"
     using cstep_star_frame_extend[OF cstepin, of "[(cont, dst, caller)]"] teq by simp
   have "csim \<Pi> g (seq_after (Seq inner' Restore) afters, s', fz' @ [Frame caller dst])
@@ -670,8 +670,8 @@ theorem csim_step:
   assumes SIM: "csim \<Pi> g (c, s, frs) (v, t, stk)"
       and PC: "procs_embedded \<Pi> g"
       and WF: "return_safe c"
-      and STEP: "pstep source_global \<Pi> (c, s, frs) src'"
-  shows "\<exists>cfg'. star (cstep source_global g) (v, t, stk) cfg' \<and> csim \<Pi> g src' cfg'"
+      and STEP: "pstep gs \<Pi> (c, s, frs) src'"
+  shows "\<exists>cfg'. star (cstep gs g) (v, t, stk) cfg' \<and> csim \<Pi> g src' cfg'"
 proof -
   consider (call) "head_call c" | (ret) "head_return c" | (returning) "is_returning c"
     | (intra) "\<not> head_call c" "\<not> head_return c" "\<not> is_returning c" by blast
@@ -699,10 +699,10 @@ qed
 
 lemma csim_run:
   assumes PC: "procs_embedded \<Pi> g"
-      and RUN: "star (pstep source_global \<Pi>) sc sc'"
+      and RUN: "star (pstep gs \<Pi>) sc sc'"
       and SIM: "csim \<Pi> g sc dg"
       and WF: "return_safe (fst sc)"
-  shows "\<exists>dg'. star (cstep source_global g) dg dg' \<and> csim \<Pi> g sc' dg'"
+  shows "\<exists>dg'. star (cstep gs g) dg dg' \<and> csim \<Pi> g sc' dg'"
   using RUN SIM WF
 proof (induction arbitrary: dg rule: star.induct)
   case (refl a)
@@ -715,17 +715,17 @@ next
   obtain v0 t0 k0 where dgd: "dg = (v0, t0, k0)" by (cases dg)
   have SIMa: "csim \<Pi> g (c0, s0, f0) (v0, t0, k0)" using step.prems(1) a dgd by simp
   have WFa: "return_safe c0" using step.prems(2) a by simp
-  have STEP: "pstep source_global \<Pi> (c0, s0, f0) (c1, s1, f1)" using step.hyps(1) a b by simp
+  have STEP: "pstep gs \<Pi> (c0, s0, f0) (c1, s1, f1)" using step.hyps(1) a b by simp
   from csim_step[OF SIMa PC WFa STEP] obtain dg1 where
-    run1: "star (cstep source_global g) (v0, t0, k0) dg1"
+    run1: "star (cstep gs g) (v0, t0, k0) dg1"
     and sim1: "csim \<Pi> g (c1, s1, f1) dg1" by blast
   have bodies: "\<And>p decl. \<Pi> p = Some decl \<Longrightarrow> source_com (body decl)"
     using procs_embedded_source_com[OF PC] .
   have WFb: "return_safe (fst b)" using return_safe_pstep[OF bodies STEP WFa] b by simp
   have sim1b: "csim \<Pi> g b dg1" using sim1 b by simp
   from step.IH[OF sim1b WFb] obtain dg' where
-    run2: "star (cstep source_global g) dg1 dg'" and sim2: "csim \<Pi> g cc dg'" by blast
-  from run1 run2 have "star (cstep source_global g) (v0, t0, k0) dg'" by (rule star_trans)
+    run2: "star (cstep gs g) dg1 dg'" and sim2: "csim \<Pi> g cc dg'" by blast
+  from run1 run2 have "star (cstep gs g) (v0, t0, k0) dg'" by (rule star_trans)
   with sim2 show ?case using dgd by blast
 qed
 
@@ -733,15 +733,15 @@ theorem csim_star:
   assumes SIM: "csim \<Pi> g (c, s, frs) (v, t, stk)"
       and PC: "procs_embedded \<Pi> g"
       and WF: "return_safe c"
-      and RUN: "star (pstep source_global \<Pi>) (c, s, frs) src'"
-  shows "\<exists>cfg'. star (cstep source_global g) (v, t, stk) cfg' \<and> csim \<Pi> g src' cfg'"
+      and RUN: "star (pstep gs \<Pi>) (c, s, frs) src'"
+  shows "\<exists>cfg'. star (cstep gs g) (v, t, stk) cfg' \<and> csim \<Pi> g src' cfg'"
   using csim_run[OF PC RUN SIM] WF by simp
 
 section \<open>The static certificate for a whole compiled program\<close>
 
 text \<open>The static source contract establishes the runtime return guard for the root activation.\<close>
 lemma wf_compile_input_return_safe:
-  assumes "wf_compile_input source_global \<Pi> ps mnm main"
+  assumes "wf_compile_input gs \<Pi> ps mnm main"
   shows "return_safe main"
   using wf_compile_inputD(8)[OF assms] wf_compile_inputD(4)[OF assms]
   by (rule return_safe_if_no_return)
@@ -755,7 +755,7 @@ text \<open>
   forever, is what closes the static side of the simulation.
 \<close>
 theorem procs_embedded_compile_prog:
-  assumes wf: "wf_compile_input source_global \<Pi> ps mnm main"
+  assumes wf: "wf_compile_input gs \<Pi> ps mnm main"
   shows "procs_embedded \<Pi> (compile_prog \<Pi> ps mnm main)"
   unfolding procs_embedded_def
 proof (intro allI impI)
